working on second volume

plf/Equiv.v
@@ -10,3 +10,61 @@ From Coq Require Import Lists.List.
 From Coq Require Import Logic.FunctionalExtensionality.
 Import ListNotations.
 From PLF Require Export Imp.
+
+Definition aequiv (a1 a2 : aexp) : Prop :=
+  forall (st : state),
+    aeval st a1 = aeval st a2.
+
+Definition bequiv (b1 b2 : bexp) : Prop :=
+  forall (st : state),
+    beval st b1 = beval st b2.
+
+Theorem aequiv_example : aequiv <{X - X}> <{ 0 }>.
+Proof.
+  intros st. simpl. lia.
+Qed.
+
+Theorem bequiv_example : bequiv <{X - X = 0}> <{ true }>.
+Proof.
+  intros st.
+  unfold beval.
+  rewrite aequiv_example.
+  reflexivity.
+Qed.
+
+Definition cequiv (c1 c2 : com) : Prop :=
+  forall (st st' : state),
+    (st =[ c1 ]=> st') <-> (st =[ c2 ]=> st').
+
+Theorem skip_left : forall c,
+    cequiv
+    <{ skip; c }>
+    c.
+Proof.
+  intros c st st'.
+  split. intros H.
+  - inversion H. subst.
+    inversion H2. subst.
+    assumption.
+  - apply E_Seq.
+    apply E_Skip.
+Qed.
+
+Check E_Seq.
+Check E_Skip.
+
+Theorem skip_right : forall c,
+    cequiv
+    <{ c; skip }>
+    c.
+Proof.
+  intros c st st'.
+  split. intros H.
+  - inversion H. subst.
+    inversion H5. subst.
+    assumption.
+  - assert (H: st' =[ skip ]=> st').{
+      apply E_Skip.
+    }.
+
+
