plf/Smallstep.v
@@ -1,0 +1,19 @@
+Set Warnings "-notation-overridden,-parsing".
+From Coq Require Import Arith.Arith.
+From Coq Require Import Arith.EqNat.
+From Coq Require Import Init.Nat.
+From Coq Require Import Lia.
+From Coq Require Import Lists.List.
+Import ListNotations.
+From PLF Require Import Maps.
+From PLF Require Import Imp.
+
+Inductive tm : Type :=
+| C : nat -> tm
+| P : tm -> tm -> tm.
+
+Fixpoint evalF (t : tm) : nat :=
+  match t with
+  | C n => n
+  | P t1 t2 => evalF t1 + evalF t2
+  end.
